theories/locks/lambdalock/langdef.v
@@ -1,0 +1,283 @@
+From cgraphs.locks.lambdalock Require Export langtools.
+
+(* Expressions and values *)
+(* ---------------------- *)
+
+Inductive expr :=
+  | Val : val -> expr
+  | Var : string -> expr
+  | Fun : string -> expr -> expr
+  | App : expr -> expr -> expr
+  | Unit : expr
+  | Pair : expr -> expr -> expr
+  | LetPair : expr -> expr -> expr
+  | Sum : nat -> expr -> expr
+  | MatchSum n : expr -> (fin n -> expr) -> expr
+  (* Barriers *)
+  | ForkBarrier : expr -> expr
+  (* Locks *)
+  | NewLock : expr -> expr
+  | ForkLock : expr -> expr -> expr
+  | Acquire : expr -> expr
+  | Release : expr -> expr -> expr
+  | Wait : expr -> expr
+  | Drop : expr -> expr
+with val :=
+  | FunV : string -> expr -> val
+  | UnitV : val
+  | PairV : val -> val -> val
+  | SumV : nat -> val -> val
+  | BarrierV : nat -> val
+  | LockV : nat -> val.
+
+
+(* Type system *)
+(* ----------- *)
+
+Inductive linearity := Lin | Unr.
+
+Inductive lockstate := Opened | Closed.
+Inductive lockownership := Owner | Client.
+Definition lockcap : Type := lockownership * lockstate.
+Inductive lockownership_split : lockownership -> lockownership -> lockownership -> Prop :=
+  | lo_split_1 : lockownership_split Owner Client Owner
+  | lo_split_2 : lockownership_split Owner Owner Client
+  | lo_split_3 : lockownership_split Client Client Client.
+Inductive lockstate_split : lockstate -> lockstate -> lockstate -> Prop :=
+  | ls_split_1 : lockstate_split Opened Closed Opened
+  | ls_split_2 : lockstate_split Opened Opened Closed
+  | ls_split_3 : lockstate_split Closed Closed Closed.
+Definition lockcap_split l1 l2 l3 :=
+  lockownership_split l1.1 l2.1 l3.1 ∧ lockstate_split l1.2 l2.2 l3.2.
+
+CoInductive type :=
+  | FunT : linearity -> type -> type -> type
+  | UnitT : type
+  | PairT : type -> type -> type
+  | SumT n : (fin n -> type) -> type
+  | LockT : lockcap -> type -> type.
+
+CoInductive unr : type -> Prop :=
+  | Fun_unr t1 t2 : unr (FunT Unr t1 t2)
+  | Unit_unr : unr UnitT
+  | Pair_unr t1 t2 : unr t1 -> unr t2 -> unr (PairT t1 t2)
+  | Sum_unr n ts : (∀ i, unr (ts i)) -> unr (SumT n ts).
+
+(* We define linear environment splitting here.
+   On paper this is implicit in Γ1,Γ2 ⊢ e : A.
+   In Coq we have to explicitly say env_split Γ Γ1 Γ2, and typed Γ e A. *)
+Definition env := gmap string type.
+
+Definition env_unr (Γ : env) :=
+  ∀ x t, Γ !! x = Some t -> unr t.
+
+Definition disj (Γ1 Γ2 : env) :=
+  ∀ i t1 t2, Γ1 !! i = Some t1 -> Γ2 !! i = Some t2 -> t1 = t2 ∧ unr t1.
+
+Definition env_split (Γ : env) (Γ1 : env) (Γ2 : env) :=
+  Γ = Γ1 ∪ Γ2 ∧ disj Γ1 Γ2.
+
+Definition env_bind (Γ' : env) (x : string) (t : type) (Γ : env) :=
+  Γ' = <[ x := t ]> Γ ∧ ∀ t', Γ !! x = Some t' -> unr t'.
+
+Definition env_var (Γ : env) (x : string) (t : type) :=
+  ∃ Γ', Γ = <[ x := t ]> Γ' ∧ env_unr Γ'.
+
+
+Inductive typed : env -> expr -> type -> Prop :=
+  (* Base language *)
+  | Var_typed Γ x t :
+    env_var Γ x t ->
+    typed Γ (Var x) t
+  | Fun_typed Γ Γ' x e t1 t2 l :
+    env_bind Γ' x t1 Γ ->
+    (l = Unr -> env_unr Γ) ->
+    typed Γ' e t2 ->
+    typed Γ (Fun x e) (FunT l t1 t2)
+  | App_typed Γ Γ1 Γ2 e1 e2 t1 t2 l :
+    env_split Γ Γ1 Γ2 ->
+    typed Γ1 e1 (FunT l t1 t2) ->
+    typed Γ2 e2 t1 ->
+    typed Γ (App e1 e2) t2
+  | Unit_typed Γ :
+    env_unr Γ ->
+    typed Γ Unit UnitT
+  | Pair_typed Γ Γ1 Γ2 e1 e2 t1 t2 :
+    env_split Γ Γ1 Γ2 ->
+    typed Γ1 e1 t1 ->
+    typed Γ2 e2 t2 ->
+    typed Γ (Pair e1 e2) (PairT t1 t2)
+  | LetPair_typed Γ Γ1 Γ2 e1 e2 t1 t2 t :
+    env_split Γ Γ1 Γ2 ->
+    typed Γ1 e1 (PairT t1 t2) ->
+    typed Γ2 e2 (FunT Lin t1 (FunT Lin t2 t)) ->
+    typed Γ (LetPair e1 e2) t
+  | Sum_typed Γ n (ts : fin n -> type) i e :
+    typed Γ e (ts i) ->
+    typed Γ (Sum i e) (SumT n ts)
+  | MatchSumN_typed n Γ Γ1 Γ2 t (ts : fin n -> type) es e :
+    env_split Γ Γ1 Γ2 ->
+    (n = 0 -> env_unr Γ2) ->
+    typed Γ1 e (SumT n ts) ->
+    (∀ i, typed Γ2 (es i) (FunT Lin (ts i) t)) ->
+    typed Γ (MatchSum n e es) t
+  (* Barriers *)
+  | Fork_typed Γ e t1 t2 :
+    typed Γ e (FunT Lin (FunT Lin t2 t1) UnitT) ->
+    typed Γ (ForkBarrier e) (FunT Lin t1 t2)
+  (* Locks *)
+  | NewLock_typed Γ e t :
+    typed Γ e t ->
+    typed Γ (NewLock e) (LockT (Owner,Closed) t)
+  | ForkLock_typed Γ Γ1 Γ2 e1 e2 t l1 l2 l3 :
+    env_split Γ Γ1 Γ2 ->
+    lockcap_split l1 l2 l3 ->
+    typed Γ1 e1 (LockT l1 t) ->
+    typed Γ2 e2 (FunT Lin (LockT l2 t) UnitT) ->
+    typed Γ (ForkLock e1 e2) (LockT l3 t)
+  | Acquire_typed Γ e t lo :
+    typed Γ e (LockT (lo,Closed) t) ->
+    typed Γ (Acquire e) (PairT (LockT (lo,Opened) t) t)
+  | Release_typed Γ Γ1 Γ2 e1 e2 t lo :
+    env_split Γ Γ1 Γ2 ->
+    typed Γ1 e1 (LockT (lo,Opened) t) ->
+    typed Γ2 e2 t ->
+    typed Γ (Release e1 e2) (LockT (lo,Closed) t)
+  | Wait_typed Γ e t :
+    typed Γ e (LockT (Owner,Closed) t) ->
+    typed Γ (Wait e) t
+  | Drop_typed Γ e t :
+    typed Γ e (LockT (Client,Closed) t) ->
+    typed Γ (Drop e) UnitT.
+
+
+(* Operational semantics *)
+(* --------------------- *)
+
+Definition subst (x:string) (a:val) := fix rec e :=
+  match e with
+  | Val _ => e
+  | Var x' => if decide (x = x') then Val a else e
+  | Fun x' e => Fun x' (if decide (x = x') then e else rec e)
+  | App e1 e2 => App (rec e1) (rec e2)
+  | Unit => Unit
+  | Pair e1 e2 => Pair (rec e1) (rec e2)
+  | LetPair e1 e2 => LetPair (rec e1) (rec e2)
+  | Sum n e => Sum n (rec e)
+  | MatchSum n e1 e2 => MatchSum n (rec e1) (rec ∘ e2)
+  | ForkBarrier e => ForkBarrier (rec e)
+  | NewLock e => NewLock (rec e)
+  | ForkLock e1 e2 => ForkLock (rec e1) (rec e2)
+  | Acquire e => Acquire (rec e)
+  | Release e1 e2 => Release (rec e1) (rec e2)
+  | Wait e => Wait (rec e)
+  | Drop e => Drop (rec e)
+  end.
+
+Inductive pure_step : expr -> expr -> Prop :=
+  | Fun_step x e :
+    pure_step (Fun x e) (Val $ FunV x e)
+  | App_step x e a :
+    pure_step (App (Val $ FunV x e) (Val a)) (subst x a e)
+  | Unit_step :
+    pure_step Unit (Val $ UnitV)
+  | Pair_step v1 v2 :
+    pure_step (Pair (Val v1) (Val v2)) (Val $ PairV v1 v2)
+  | LetPair_step v1 v2 e:
+    pure_step (LetPair (Val $ PairV v1 v2) e) (App (App e (Val v1)) (Val v2))
+  | Sum_step n v :
+    pure_step (Sum n (Val v)) (Val $ SumV n v)
+  | MatchSum_step n (i : fin n) v es :
+    pure_step (MatchSum n (Val $ SumV i v) es) (App (es i) (Val v)).
+
+Inductive ctx1 : (expr -> expr) -> Prop :=
+  | Ctx_App_l e : ctx1 (λ x, App x e)
+  | Ctx_App_r e : ctx1 (λ x, App e x)
+  | Ctx_Pair_l e : ctx1 (λ x, Pair x e)
+  | Ctx_Pair_r e : ctx1 (λ x, Pair e x)
+  | Ctx_LetPair e : ctx1 (λ x, LetPair x e)
+  | Ctx_Sum i : ctx1 (λ x, Sum i x)
+  | Ctx_MatchSum n es : ctx1 (λ x, MatchSum n x es)
+  | Ctx_ForkBarrier : ctx1 (λ x, ForkBarrier x)
+  | Ctx_NewLock : ctx1 (λ x, NewLock x)
+  | Ctx_ForkLock_l e : ctx1 (λ x, ForkLock x e)
+  | Ctx_ForkLock_r e : ctx1 (λ x, ForkLock e x)
+  | Ctx_Acquire : ctx1 (λ x, Acquire x)
+  | Ctx_Release_l e : ctx1 (λ x, Release x e)
+  | Ctx_Release_r e : ctx1 (λ x, Release e x)
+  | Ctx_Wait : ctx1 (λ x, Wait x)
+  | Ctx_Drop : ctx1 (λ x, Drop x).
+
+Inductive ctx : (expr -> expr) -> Prop :=
+  | Ctx_id : ctx id
+  | Ctx_comp k1 k2 : ctx1 k1 -> ctx k2 -> ctx (k1 ∘ k2).
+
+Inductive obj := Thread (e : expr) | Barrier | Lock (refcnt : nat) (o : option val).
+Definition cfg := gmap nat obj.
+
+Inductive local_step : nat -> cfg -> cfg -> Prop :=
+  (* Base language *)
+  | Pure_step i k e e' :
+    ctx k -> pure_step e e' ->
+    local_step i {[ i := Thread (k e) ]} {[ i := Thread (k e') ]}
+  | Exit_step i :
+    local_step i {[ i := Thread (Val UnitV) ]} ∅
+  (* Barriers *)
+  | Fork_step i j n k v :
+    i ≠ j -> i ≠ n -> j ≠ n -> ctx k ->
+    local_step i {[ i := Thread (k (ForkBarrier (Val v))) ]}
+                 {[ i := Thread (k (Val $ BarrierV n));
+                    j := Thread (App (Val v) (Val $ BarrierV n));
+                    n := Barrier ]}
+  | Sync_step i j n k1 k2 v1 v2 :
+    i ≠ j -> i ≠ n -> j ≠ n -> ctx k1 -> ctx k2 ->
+    local_step n {[ i := Thread (k1 (App (Val $ BarrierV n) (Val v1)));
+                    j := Thread (k2 (App (Val $ BarrierV n) (Val v2)));
+                    n := Barrier ]}
+                 {[ i := Thread (k1 $ Val v2);
+                    j := Thread (k2 $ Val v1) ]}
+  (* Locks *)
+  | NewLock_step v k n i:
+    i ≠ n -> ctx k ->
+    local_step i {[ i := Thread (k (NewLock (Val v))) ]}
+                 {[ i := Thread (k (Val $ LockV n));
+                    n := Lock 0 (Some v) ]}
+  | ForkLock_step v o k i j n refcnt :
+    i ≠ j -> i ≠ n -> j ≠ n -> ctx k ->
+    local_step n {[ i := Thread (k (ForkLock (Val $ LockV n) (Val v)));
+                    n := Lock refcnt o ]}
+                 {[ i := Thread (k (Val $ LockV n));
+                    j := Thread (App (Val v) (Val $ LockV n));
+                    n := Lock (S refcnt) o ]}
+  | Acquire_step v k i n refcnt :
+    i ≠ n -> ctx k ->
+    local_step n {[ i := Thread (k (Acquire (Val $ LockV n)));
+                    n := Lock refcnt (Some v) ]}
+                 {[ i := Thread (k (Val $ PairV (LockV n) v));
+                    n := Lock refcnt None ]}
+  | Release_step v k i n refcnt :
+    i ≠ n -> ctx k ->
+    local_step n {[ i := Thread (k (Release (Val $ LockV n) (Val v)));
+                    n := Lock refcnt None ]}
+                 {[ i := Thread (k (Val $ LockV n));
+                    n := Lock refcnt (Some v) ]}
+  | Wait_step v k i n :
+    i ≠ n -> ctx k ->
+    local_step n {[ i := Thread (k (Wait (Val $ LockV n)));
+                    n := Lock 0 (Some v) ]}
+                 {[ i := Thread (k (Val v)) ]}
+  | Drop_step o k i n refcnt :
+    i ≠ n -> ctx k ->
+    local_step n {[ i := Thread (k (Drop (Val $ LockV n)));
+                    n := Lock (S refcnt) o ]}
+                 {[ i := Thread (k (Val $ UnitV));
+                    n := Lock refcnt o ]}.
+
+Inductive step : nat -> cfg -> cfg -> Prop :=
+  | Frame_step ρ ρ' ρf i :
+    ρ ##ₘ ρf -> ρ' ##ₘ ρf ->
+    local_step i ρ ρ' -> step i (ρ ∪ ρf) (ρ' ∪ ρf).
+
+Definition step' ρ ρ' := ∃ i, step i ρ ρ'.
+Definition steps := rtc step'.
+
