theories/locks/lambdalock/rtypesystem.v
@@ -1,0 +1,554 @@
+From cgraphs.locks.lambdalock Require Export langdef definitions.
+
+Notation vertex := nat.
+Inductive label : Type :=
+  | BarrierLabel (b : bool) (t1 t2 : type)
+  | LockLabel (c : lockcap) (t : type).
+
+Canonical Structure typeO := leibnizO type.
+Canonical Structure labelO := leibnizO label.
+
+Notation rProp := (hProp vertex labelO).
+
+Definition linbox l (P : rProp) : rProp :=
+  match l with
+  | Lin => P
+  | Unr => □ P
+  end.
+
+Fixpoint rtyped (Γ : env) e t : rProp :=
+  match e with
+  | Val v => ⌜⌜ env_unr Γ ⌝⌝ ∗ vtyped v t
+  | Var x => ⌜⌜ env_var Γ x t ⌝⌝
+  | Fun x e =>
+      ∃ l t1 t2, ⌜⌜ t = FunT l t1 t2 ⌝⌝  ∗
+      ∃ Γ', ⌜⌜ env_bind Γ' x t1 Γ ∧ (l = Unr -> env_unr Γ) ⌝⌝ ∗
+      linbox l (rtyped Γ' e t2)
+  | App e1 e2 =>
+      ∃ Γ1 Γ2, ⌜⌜ env_split Γ Γ1 Γ2 ⌝⌝ ∗
+      ∃ t1 l,
+      rtyped Γ1 e1 (FunT l t1 t) ∗
+      rtyped Γ2 e2 t1
+  | Unit => ⌜⌜ t = UnitT ∧ env_unr Γ ⌝⌝
+  | Pair e1 e2 =>
+      ∃ Γ1 Γ2, ⌜⌜ env_split Γ Γ1 Γ2 ⌝⌝ ∗
+      ∃ t1 t2, ⌜⌜ t = PairT t1 t2 ⌝⌝ ∗
+      rtyped Γ1 e1 t1 ∗ rtyped Γ2 e2 t2
+  | LetPair e1 e2 =>
+      ∃ Γ1 Γ2, ⌜⌜ env_split Γ Γ1 Γ2 ⌝⌝ ∗
+      ∃ t1 t2,
+      rtyped Γ1 e1 (PairT t1 t2) ∗
+      rtyped Γ2 e2 (FunT Lin t1 (FunT Lin t2 t))
+  | Sum i e =>
+      ∃ n (ts : fin n -> type) (i' : fin n), ⌜⌜ t = SumT n ts ⌝⌝ ∗ ⌜⌜ i = i' ⌝⌝ ∗
+      rtyped Γ e (ts i')
+  | MatchSum n e es =>
+      ∃ Γ1 Γ2, ⌜⌜ env_split Γ Γ1 Γ2 ∧ (n = 0 -> env_unr Γ2)⌝⌝ ∗
+      ∃ ts,
+      rtyped Γ1 e (SumT n ts) ∗
+      if decide (n=0) then ⌜⌜ env_unr Γ2 ⌝⌝ else (∀ i, rtyped Γ2 (es i) (FunT Lin (ts i) t))
+  | ForkBarrier e =>
+      ∃ t1 t2, ⌜⌜ t = FunT Lin t1 t2 ⌝⌝ ∗
+      rtyped Γ e (FunT Lin (FunT Lin t2 t1) UnitT)
+  | NewLock e =>
+      ∃ t', ⌜⌜ t = LockT (Owner,Closed) t' ⌝⌝ ∗
+      rtyped Γ e t'
+  | ForkLock e1 e2 =>
+      ∃ Γ1 Γ2, ⌜⌜ env_split Γ Γ1 Γ2 ⌝⌝ ∗
+      ∃ t' l1 l2 l3, ⌜⌜ t = LockT l3 t' ∧ lockcap_split l1 l2 l3 ⌝⌝ ∗
+      rtyped Γ1 e1 (LockT l1 t') ∗
+      rtyped Γ2 e2 (FunT Lin (LockT l2 t') UnitT)
+  | Acquire e =>
+      ∃ lo t', ⌜⌜ t = PairT (LockT (lo,Opened) t') t' ⌝⌝ ∗
+      rtyped Γ e (LockT (lo,Closed) t')
+  | Release e1 e2 =>
+      ∃ Γ1 Γ2, ⌜⌜ env_split Γ Γ1 Γ2 ⌝⌝ ∗
+      ∃ lo t', ⌜⌜ t = LockT (lo,Closed) t' ⌝⌝ ∗
+      rtyped Γ1 e1 (LockT (lo,Opened) t') ∗
+      rtyped Γ2 e2 t'
+  | Wait e =>
+      rtyped Γ e (LockT (Owner,Closed) t)
+  | Drop e =>
+      ∃ t', ⌜⌜ t = UnitT ⌝⌝ ∗
+      rtyped Γ e (LockT (Client,Closed) t')
+  end
+with vtyped v t :=
+  match v with
+  | FunV x e =>
+      ∃ l t1 t2, ⌜⌜ t = FunT l t1 t2 ⌝⌝ ∗ linbox l (rtyped {[ x := t1 ]} e t2)
+  | UnitV => ⌜⌜ t = UnitT ⌝⌝
+  | PairV v1 v2 =>
+      ∃ t1 t2, ⌜⌜ t = PairT t1 t2 ⌝⌝ ∗
+      vtyped v1 t1 ∗ vtyped v2 t2
+  | SumV i v =>
+      ∃ n ts (i' : fin n), ⌜⌜ t = SumT n ts ∧ i = i' ⌝⌝ ∗
+      vtyped v (ts i')
+  | BarrierV k =>
+      ∃ t1 t2, ⌜⌜ t = FunT Lin t1 t2 ⌝⌝ ∗
+      own_out k ((BarrierLabel false t1 t2) : labelO)
+  | LockV k =>
+      ∃ l t', ⌜⌜ t = LockT l t' ⌝⌝ ∗
+      own_out k ((LockLabel l t') : labelO)
+  end.
+
+Lemma typed_rtyped Γ e t :
+  ⌜⌜ typed Γ e t ⌝⌝ -∗ rtyped Γ e t.
+Proof.
+  iIntros (H).
+  iInduction e as [] "IH" forall (t Γ H);
+  inv H; simpl; eauto; repeat iExists _; try iSplitL; eauto;
+  repeat iExists _; try iSplitL; eauto; try iSplitL;
+  try destruct l; try case_decide; repeat iIntros (?); subst; eauto;
+  try solve [ iApply ("IH" with "[%]") || iApply ("IH1" with "[%]"); eauto].
+Qed.
+
+(* From stdpp's naive_solver *)
+Ltac simp :=
+  repeat match goal with
+  (**i solve the goal *)
+  | |- _ => fast_done
+  (**i intros *)
+  | |- ∀ _, _ => intro
+  (**i simplification of assumptions *)
+  | H : False |- _ => destruct H
+  | H : _ ∧ _ |- _ =>
+     (* Work around bug https://coq.inria.fr/bugs/show_bug.cgi?id=2901 *)
+     let H1 := fresh in let H2 := fresh in
+     destruct H as [H1 H2]; try clear H
+  | H : ∃ _, _  |- _ =>
+     let x := fresh in let Hx := fresh in
+     destruct H as [x Hx]; try clear H
+  | H : ?P → ?Q, H2 : ?P |- _ => specialize (H H2)
+  | H : Is_true (bool_decide _) |- _ => apply (bool_decide_unpack _) in H
+  | H : Is_true (_ && _) |- _ => apply andb_True in H; destruct H
+  (**i simplify and solve equalities *)
+  | |- _ => progress simplify_eq/=
+  (**i operations that generate more subgoals *)
+  (* | |- _ ∧ _ => split *)
+  (* | |- Is_true (bool_decide _) => apply (bool_decide_pack _) *)
+  (* | |- Is_true (_ && _) => apply andb_True; split *)
+  (* | H : _ ∨ _ |- _ => *)
+     (* let H1 := fresh in destruct H as [H1|H1]; try clear H *)
+  (* | H : Is_true (_ || _) |- _ => *)
+     (* apply orb_True in H; let H1 := fresh in destruct H as [H1|H1]; try clear H *)
+  (**i solve the goal using the user supplied tactic *)
+  end.
+
+Ltac iDestr H := repeat (iDestruct "H" as %? || iDestruct H as (?) H).
+Ltac iSpl := repeat (iExists _ || iSplit || iIntros (?)).
+
+Lemma unrestricted_box v t :
+  unr t -> vtyped v t -∗ □ vtyped v t.
+Proof.
+  iIntros (H) "H".
+  iInduction v as [] "IH" forall (t H); simpl;
+  iDestr "H"; simp; inv H; simp; eauto.
+  - iDestruct "H" as "#H". iModIntro. eauto.
+  - iDestruct "H" as "[H1 H2]".
+    iDestruct ("IH" with "[%] H1") as "H1"; first done.
+    iDestruct ("IH1" with "[%] H2") as "H2"; first done.
+    iDestruct "H1" as "#H1".
+    iDestruct "H2" as "#H2".
+    iModIntro. repeat (iExists _ || iSplitL); eauto.
+  - iDestruct ("IH" with "[%] H") as "H"; first done.
+    iDestruct "H" as "#H". iModIntro. eauto.
+Qed.
+
+
+Definition substR (Γ : env) x v := from_option (vtyped v) emp%I (Γ !! x).
+
+Ltac sdec := repeat case_decide; simplify_eq; simpl in *; eauto; try done.
+Ltac smap := repeat (rewrite lookup_alter_spec || rewrite lookup_union || rewrite lookup_insert_spec || rewrite lookup_delete_spec || sdec).
+
+Lemma env_unr_substR Γ x v :
+  env_unr Γ -> substR Γ x v ⊢ emp.
+Proof.
+  rewrite /env_unr /substR.
+  destruct (Γ !! x) eqn:E; simp.
+  rewrite unrestricted_box; eauto.
+Qed.
+
+Lemma env_split_substR Γ Γ1 Γ2 x v :
+  env_split Γ Γ1 Γ2 -> substR Γ x v ⊢ substR Γ1 x v ∗ substR Γ2 x v.
+Proof.
+  rewrite /env_split /substR. simp.
+  rewrite lookup_union.
+  destruct (Γ1 !! x) eqn:E;
+  destruct (Γ2 !! x) eqn:F; rewrite ?E ?F; simpl; eauto.
+  edestruct (H1 x); eauto. simp.
+  iIntros "H".
+  iDestruct (unrestricted_box with "H") as "H"; eauto.
+  iDestruct "H" as "#H". iSplitL; eauto.
+Qed.
+
+Lemma env_var_substR Γ x y v t :
+  env_var Γ y t ->
+  substR Γ x v ⊢ if decide (x = y) then vtyped v t else emp.
+Proof.
+  rewrite /env_var /substR. simp. smap.
+  destruct (_!!_) eqn:E; simp.
+  rewrite unrestricted_box; eauto.
+Qed.
+
+Lemma env_bind_substR Γ Γ' l x y v t :
+  (l = Unr -> env_unr Γ) -> env_bind Γ' y t Γ ->
+  substR Γ x v ⊢ if decide (x = y) then emp else linbox l (substR Γ' x v).
+Proof.
+  rewrite /env_bind /substR. simp. smap.
+  - destruct (Γ !! y) eqn:E; simpl; eauto.
+    rewrite unrestricted_box; eauto.
+  - destruct (Γ !! x) eqn:E; rewrite ?E; destruct l; eauto; simpl.
+    rewrite {1}unrestricted_box; eauto.
+    eapply H; eauto.
+Qed.
+
+Lemma env_unr_delete Γ x :
+  env_unr Γ -> env_unr (delete x Γ).
+Proof.
+  rewrite /env_unr. intros ???. smap.
+Qed.
+
+Lemma env_split_delete Γ Γ1 Γ2 x :
+  env_split Γ Γ1 Γ2 -> env_split (delete x Γ) (delete x Γ1) (delete x Γ2).
+Proof.
+  rewrite /env_split /disj. simp.
+  split; [apply delete_union|].
+  intros ???. smap.
+Qed.
+
+Lemma env_var_delete y x Γ t :
+  env_var Γ x t -> if decide (y = x) then env_unr (delete y Γ) else env_var (delete y Γ) x t.
+Proof.
+  rewrite /env_var /env_unr. simp. smap.
+  - simp. revert H. smap.
+  - exists (delete y H0). split.
+    + apply map_eq. intro. smap.
+    + intros ??. smap.
+Qed.
+
+Lemma env_bind_delete x y t Γ Γ' :
+  env_bind Γ' x t Γ ->
+  env_bind (if decide (y = x) then Γ' else delete y Γ') x t (delete y Γ).
+Proof.
+  rewrite /env_bind. simp.
+  split.
+  - apply map_eq. intro. smap.
+  - intro. smap.
+Qed.
+
+Lemma env_unr_empty :
+  env_unr ∅.
+Proof.
+  rewrite /env_unr. intros ??. smap.
+Qed.
+
+Lemma env_split_empty Γ1 Γ2 :
+  env_split ∅ Γ1 Γ2 <-> Γ1 = ∅ ∧ Γ2 = ∅.
+Proof.
+  rewrite /env_split.
+  split. simp.
+  - symmetry in H0.
+    pose proof (map_positive_l _ _ H0). subst.
+    rewrite left_id in H0. subst. eauto.
+  - simp. rewrite left_id. split; eauto.
+    rewrite /disj. intros ??. smap.
+Qed.
+
+Lemma env_var_empty x t :
+  env_var ∅ x t <-> False.
+Proof.
+  rewrite /env_var. split; simp.
+  rewrite map_eq_iff in H. specialize (H x). revert H. smap.
+Qed.
+
+Lemma env_bind_empty Γ x t1 :
+  env_bind Γ x t1 ∅ <-> Γ = {[ x := t1 ]}.
+Proof.
+  rewrite /env_bind. repeat split; simp.
+Qed.
+
+
+Lemma linbox_mono P Q l :
+  □ (P -∗ Q) -∗ linbox l P -∗ linbox l Q.
+Proof.
+  iIntros "#H P".
+  destruct l; simpl; [|iDestruct "P" as "#P"; iModIntro];
+  iApply "H"; done.
+Qed.
+
+Lemma linbox_sep P Q l :
+  linbox l P ∗ linbox l Q ⊢ linbox l (P ∗ Q).
+Proof.
+  destruct l; simpl; eauto.
+  iIntros "[#H #R]". iModIntro.
+  iSplitL; eauto.
+Qed.
+
+
+Lemma substitution Γ x v e t :
+  substR Γ x v ∗
+  rtyped Γ e t -∗
+  rtyped (delete x Γ) (subst x v e) t.
+Proof.
+  iIntros "RH".
+  iInduction e as [] "IH" forall (Γ t); simpl;
+  iDestruct "RH" as "[R H]"; iDestr "H"; try iDestruct "H" as "[H Q]"; simp.
+  - rewrite env_unr_substR //. iSpl; eauto using env_unr_delete.
+  - rewrite env_var_substR //.
+    eapply (env_var_delete x) in H.
+    case_decide; subst; simpl; iFrame; iPureIntro; eauto.
+  - iExists _,_,_. iSplit; first done.
+    iExists _. iSplit; eauto 6 using env_bind_delete, env_unr_delete.
+    rewrite env_bind_substR; eauto.
+    case_decide; subst; iFrame.
+    iApply linbox_mono; eauto.
+    iApply linbox_sep. iFrame.
+  - iDestruct (env_split_substR with "R") as "[R1 R2]"; eauto.
+    iSpl; eauto using env_split_delete.
+    iSplitL "H R1"; (iApply "IH" || iApply "IH1"); eauto with iFrame.
+  - rewrite env_unr_substR //.
+    eauto using env_unr_delete.
+  - iDestruct (env_split_substR with "R") as "[R1 R2]"; eauto.
+    iSpl; eauto using env_split_delete.
+    iSplitL "H R1"; (iApply "IH" || iApply "IH1"); eauto with iFrame.
+  - iDestruct (env_split_substR with "R") as "[R1 R2]"; eauto.
+    iSpl; eauto using env_split_delete.
+    iSplitL "H R1"; (iApply "IH" || iApply "IH1"); eauto with iFrame.
+  - iSpl; eauto. iApply "IH". iFrame.
+  - iDestruct (env_split_substR with "R") as "[R1 R2]"; eauto.
+    iSpl; first iPureIntro; eauto using env_split_delete, env_unr_delete.
+    case_decide; subst.
+    { iDestruct "Q" as "%". iSplit; eauto using env_unr_delete.
+      eapply env_unr_substR in H. rewrite H.
+      iApply "IH1". iFrame. }
+    iSplitL "H R1"; iSpl; (iApply "IH" || iApply "IH1"); eauto with iFrame.
+  - iSpl; eauto. (iApply "IH" || iApply "IH1"); eauto with iFrame.
+  - iSpl; eauto. iApply "IH". iFrame.
+  - iSpl; eauto using env_split_delete.
+    iDestruct (env_split_substR with "R") as "[R1 R2]"; eauto.
+    iSplitL "H R1"; (iApply "IH" || iApply "IH1"); iFrame.
+  - iSpl; eauto. iApply "IH". iFrame.
+  - iSpl; eauto using env_split_delete.
+    iDestruct (env_split_substR with "R") as "[R1 R2]"; eauto.
+    iSplitL "H R1"; (iApply "IH" || iApply "IH1"); iFrame.
+  - iSpl; eauto. iApply "IH". iFrame.
+  - iSpl; eauto. iApply "IH". iFrame.
+Qed.
+
+Fixpoint rtyped0 e t : rProp :=
+  match e with
+  | Val v => vtyped v t
+  | Var x => False
+  | Fun x e =>
+      ∃ l t1 t2, ⌜⌜ t = FunT l t1 t2 ⌝⌝ ∗
+      ∃ Γ, ⌜⌜ env_bind Γ x t1 ∅ ⌝⌝ ∗
+      linbox l (rtyped Γ e t2)
+  | App e1 e2 =>
+      ∃ t1 l,
+      rtyped0 e1 (FunT l t1 t) ∗
+      rtyped0 e2 t1
+  | Unit => ⌜⌜ t = UnitT ⌝⌝
+  | Pair e1 e2 =>
+      ∃ t1 t2, ⌜⌜ t = PairT t1 t2 ⌝⌝ ∗
+      rtyped0 e1 t1 ∗ rtyped0 e2 t2
+  | LetPair e1 e2 =>
+      ∃ t1 t2,
+      rtyped0 e1 (PairT t1 t2) ∗
+      rtyped0 e2 (FunT Lin t1 (FunT Lin t2 t))
+  | Sum i e =>
+      ∃ n (ts : fin n -> type) (i' : fin n), ⌜⌜ t = SumT n ts ⌝⌝ ∗ ⌜⌜ i = i' ⌝⌝ ∗
+      rtyped0 e (ts i')
+  | MatchSum n e es =>
+      ∃ ts,
+      rtyped0 e (SumT n ts) ∗
+      if decide (n=0) then emp else (∀ i, rtyped0 (es i) (FunT Lin (ts i) t))
+  (* Barriers *)
+  | ForkBarrier e =>
+      ∃ t1 t2, ⌜⌜ t = FunT Lin t1 t2 ⌝⌝ ∗
+      rtyped0 e (FunT Lin (FunT Lin t2 t1) UnitT)
+  (* Locks *)
+  | NewLock e =>
+      ∃ t', ⌜⌜ t = LockT (Owner,Closed) t' ⌝⌝ ∗
+      rtyped0 e t'
+  | ForkLock e1 e2 =>
+      ∃ t' l1 l2 l3, ⌜⌜ t = LockT l3 t' ∧ lockcap_split l1 l2 l3 ⌝⌝ ∗
+      rtyped0 e1 (LockT l1 t') ∗
+      rtyped0 e2 (FunT Lin (LockT l2 t') UnitT)
+  | Acquire e =>
+      ∃ lo t', ⌜⌜ t = PairT (LockT (lo,Opened) t') t' ⌝⌝ ∗
+      rtyped0 e (LockT (lo,Closed) t')
+  | Release e1 e2 =>
+      ∃ lo t', ⌜⌜ t = LockT (lo,Closed) t' ⌝⌝ ∗
+      rtyped0 e1 (LockT (lo,Opened) t') ∗
+      rtyped0 e2 t'
+  | Wait e =>
+      rtyped0 e (LockT (Owner,Closed) t)
+  | Drop e =>
+      ∃ t', ⌜⌜ t = UnitT ⌝⌝ ∗
+      rtyped0 e (LockT (Client,Closed) t')
+  end.
+
+
+Lemma rtyped_rtyped0 e t :
+  rtyped ∅ e t ⊣⊢ rtyped0 e t.
+Proof.
+  revert t. induction e; intros; simpl;
+  iSplit; iIntros "H";
+  try setoid_rewrite env_split_empty;
+  try setoid_rewrite env_var_empty;
+  try setoid_rewrite env_bind_empty;
+  iDestr "H"; simp; eauto using env_unr_empty;
+  try iDestruct "H" as "[H Q]";
+  repeat (iExists _ || iSplit); eauto using env_unr_empty;
+  rewrite ?H ?IHe ?IHe1 ?IHe2; try case_decide; iFrame; eauto using env_unr_empty;
+  iIntros (?); setoid_rewrite H; eauto.
+Qed.
+
+Lemma substitution0 v t1 t2 x e :
+  vtyped v t1 ∗
+  rtyped {[ x := t1 ]} e t2 -∗
+  rtyped0 (subst x v e) t2.
+Proof.
+  rewrite -rtyped_rtyped0.
+  iIntros "[H Q]".
+  iDestruct (substitution _ x v e t2 with "[H Q]") as "H"; iFrame.
+  - rewrite /substR lookup_singleton //.
+  - rewrite delete_singleton //.
+Qed.
+
+Lemma pure_preservation e e' t :
+  pure_step e e' ->
+  rtyped0 e t -∗ rtyped0 e' t.
+Proof.
+  intros []; simpl;
+  iIntros "H";
+  try setoid_rewrite env_bind_empty;
+  repeat (iDestr "H" || iDestruct "H" as "[H ?]"); simp;
+  repeat (iExists _ || iSplit || case_decide); eauto with iFrame.
+  - iApply substitution0. iFrame. by destruct l0.
+  - subst. inv_fin i'.
+Qed.
+
+Lemma replacement1 k e B :
+  ctx1 k ->
+  rtyped0 (k e) B -∗ ∃ t, rtyped0 e t ∗ ∀ e', rtyped0 e' t -∗ rtyped0 (k e') B.
+Proof.
+  destruct 1; simpl; iIntros "H";
+  iDestr "H"; try iDestruct "H" as "[H Q]";
+  eauto 9 with iFrame.
+Qed.
+
+Lemma replacement k e B :
+  ctx k ->
+  rtyped0 (k e) B ⊣⊢ ∃ t, rtyped0 e t ∗ ∀ e', rtyped0 e' t -∗ rtyped0 (k e') B.
+Proof.
+  intros Hk.
+  iSplit; iIntros "H"; last first.
+  { iDestruct "H" as (t) "[H Q]". by iApply "Q". }
+  iInduction Hk as [] "IH" forall (B e); simpl.
+  { iExists _. iFrame. eauto. } subst.
+  iDestruct (replacement1 with "H") as (?) "[H R]"; eauto.
+  iDestruct ("IH" with "H") as (?) "[Q H]".
+  iExists _. iFrame. iIntros (?) "?".
+  iApply "R". iApply "H". done.
+Qed.
+
+
+Ltac solve_ctx := solve [iPureIntro; do 2 eexists; split; last done; eauto using ctx, ctx1].
+Ltac solve_step := solve [iPureIntro; do 2 eexists; split; eauto using Ctx_id; simp; eauto using pure_step].
+
+Ltac solve_pr := simp; solve [solve_ctx || solve_step].
+
+Inductive impure : expr -> Prop :=
+  | imp_ForkBarrier v : impure (ForkBarrier (Val v))
+  | imp_NewLock v : impure (NewLock (Val v))
+  | imp_Waiting e i : expr_head_waiting e i -> impure e.
+
+Definition step_or_impure e := ∃ k e0,
+  ctx k ∧ e = k e0 ∧ ((∃ e', pure_step e0 e') ∨ impure e0).
+
+Lemma step_or_impure_ctx1 e e0 k :
+  ctx1 k -> e0 = k e -> step_or_impure e -> step_or_impure e0.
+Proof.
+  intros Hctx -> (k' & e' & Hctx' & -> & D).
+  unfold step_or_impure. eexists (k ∘ k'),_.
+  eauto using Ctx_comp.
+Qed.
+
+Lemma pure_step_or_impure e e' :
+  pure_step e e' -> step_or_impure e.
+Proof.
+  intros Hs. eexists id,_;
+  eauto using Ctx_id.
+Qed.
+
+Lemma impure_or_impure e :
+  impure e -> step_or_impure e.
+Proof.
+  intros Hi. eexists id,_;
+  eauto using Ctx_id.
+Qed.
+
+Definition is_Val e := ∃ v, e = Val v.
+
+Ltac into_val H1 H2 :=
+  iDestruct (H1 with H2) as %[[? ->]|?];
+  last by eauto using step_or_impure_ctx1, ctx1.
+
+Ltac ppdone := simp; eauto using pure_step_or_impure, pure_step, impure_or_impure, impure, expr_head_waiting.
+
+Lemma pure_progress e t :
+  rtyped0 e t -∗ ⌜ is_Val e ∨ step_or_impure e ⌝.
+Proof.
+  iIntros "H".
+  iInduction e as [] "IH" forall (t); simpl; eauto;
+  first (iLeft; unfold is_Val; by eauto); iRight.
+  (* Base language *)
+  - ppdone.
+  - iDestr "H". iDestruct "H" as "[H H1]".
+    into_val "IH" "H".
+    into_val "IH1" "H1".
+    destruct x; simpl; iDestr "H"; ppdone.
+  - ppdone.
+  - iDestr "H". iDestruct "H" as "[H H1]".
+    into_val "IH" "H".
+    into_val "IH1" "H1".
+    ppdone.
+  - iDestr "H". iDestruct "H" as "[H H1]".
+    into_val "IH" "H". simpl.
+    destruct x; simpl; iDestr "H"; ppdone.
+  - iDestr "H"; simp.
+    into_val "IH" "H". simpl.
+    ppdone.
+  - iDestr "H". iDestruct "H" as "[H H1]".
+    into_val "IH1" "H". simpl.
+    destruct x; simpl; iDestr "H";
+    ppdone.
+  (* Barriers *)
+  - iDestr "H".
+    into_val "IH" "H". ppdone.
+  (* Locks *)
+  - iDestr "H". into_val "IH" "H". ppdone.
+  - iDestr "H". iDestruct "H" as "[H H1]".
+    into_val "IH" "H".
+    into_val "IH1" "H1".
+    destruct x; simpl; iDestr "H"; simp.
+    ppdone.
+  - iDestr "H".
+    into_val "IH" "H".
+    destruct x; simpl; iDestr "H"; simp.
+    ppdone.
+  - iDestr "H". iDestruct "H" as "[H H1]".
+    into_val "IH" "H".
+    into_val "IH1" "H1".
+    destruct x; simpl; iDestr "H"; simp.
+    ppdone.
+  - iDestr "H".
+    into_val "IH" "H".
+    destruct x; simpl; iDestr "H"; simp.
+    ppdone.
+  - iDestr "H".
+    into_val "IH" "H".
+    destruct x; simpl; iDestr "H"; simp.
+    ppdone.
+Qed.
