theories/locks/lambdalock/theorems.v
@@ -1,0 +1,47 @@
+From cgraphs.locks.lambdalock Require Import invariant.
+
+
+Lemma fully_reachable_iff_deadlock_free ρ :
+  fully_reachable ρ <-> deadlock_free ρ.
+Proof.
+  split.
+  - intros Hfr s [] i si.
+    destruct (Hfr i); eauto.
+    exfalso. induction H; naive_solver.
+  - intros Hdf i. classical_left.
+    eapply (Hdf (λ i, ¬ reachable ρ i));
+    first constructor; eauto using reachable.
+Qed.
+
+Lemma fully_reachable_type_safety ρ :
+  fully_reachable ρ -> type_safety ρ.
+Proof.
+  intros Hfr i. destruct (Hfr i) as [|[]]; eauto.
+Qed.
+
+Lemma fully_reachable_global_progress ρ :
+  fully_reachable ρ -> global_progress ρ.
+Proof.
+  intros Hfr.
+  destruct (classic (∃ i, ¬ inactive ρ i)).
+  - destruct H as [i Hi]. destruct (Hfr i); first naive_solver.
+    clear Hi. right. induction H; eauto.
+  - left. intros i. apply NNPP. eauto.
+Qed.
+
+Lemma typed_full_reachability e ρ :
+  typed ∅ e UnitT -> steps {[ 0 := Thread e ]} ρ -> fully_reachable ρ.
+Proof.
+  intros Ht Hsteps.
+  assert (ginv {[ 0 := Thread e ]}) as Hinv.
+  { eapply initialization. done. }
+  induction Hsteps.
+  - eapply full_reachability. done.
+  - eapply IHHsteps. destruct H. eapply preservation; eauto.
+Qed.
+
+Lemma typed_global_progress e ρ :
+  typed ∅ e UnitT -> steps {[ 0 := Thread e ]} ρ -> global_progress ρ.
+Proof.
+  intros. eapply fully_reachable_global_progress, typed_full_reachability; done.
+Qed.
