mkmpgv.sh
@@ -1,15 +1,17 @@
-git archive HEAD -o mpgv.zip
-zip -d mpgv.zip theories/locks
-zip -d mpgv.zip theories/locks/*
-zip -d mpgv.zip theories/sessiontypes
-zip -d mpgv.zip theories/sessiontypes/*
-zip -d mpgv.zip theories/lambdabar
-zip -d mpgv.zip theories/lambdabar/*
-zip -d mpgv.zip README.md
-zip -d mpgv.zip mkmpgv.sh
-mv README.md README_tmp.md
-cp theories/multiparty/README.md README.md
-zip -r mpgv.zip README.md README.md
-rm README.md
-mv README_tmp.md README.md
+git archive HEAD -o sources.zip
+zip -d sources.zip theories/multiparty
+zip -d sources.zip theories/multiparty/*
+zip -d sources.zip theories/locks/lambdalockpp
+zip -d sources.zip theories/locks/lambdalockpp/*
+zip -d sources.zip theories/sessiontypes
+zip -d sources.zip theories/sessiontypes/*
+zip -d sources.zip theories/lambdabar
+zip -d sources.zip theories/lambdabar/*
+zip -d sources.zip README.md
+zip -d sources.zip mkmpgv.sh
+# mv README.md README_tmp.md
+# cp theories/multiparty/README.md README.md
+# zip -r sources.zip README.md README.md
+# rm README.md
+# mv README_tmp.md README.md
 # scp -P 5555 mpgv.zip artifact@localhost:mpgv.zip
