theories/locks/lambdalockpp/plan.md
@@ -1,0 +1,7 @@
+[ ] Add lockpp syntax
+[ ] Add lockpp typing rules
+[ ] Add lockpp opsem
+[ ] Update rtypesystem
+[ ] Update definitions
+[ ] Update invariant.v
+[ ] Mechanize examples
